<?xml version="1.0"?>
<rdf:RDF xmlns="http://www.theworldavatar.com/ontology/ontopowsys/PowSysFunction.owl#"
     xml:base="http://www.theworldavatar.com/ontology/ontopowsys/PowSysFunction.owl"
     xmlns:rdf="http://www.w3.org/1999/02/22-rdf-syntax-ns#"
     xmlns:terms="http://purl.org/dc/terms/"
     xmlns:owl="http://www.w3.org/2002/07/owl#"
     xmlns:xml="http://www.w3.org/XML/1998/namespace"
     xmlns:xsd="http://www.w3.org/2001/XMLSchema#"
     xmlns:rdfs="http://www.w3.org/2000/01/rdf-schema#">
    <owl:Ontology rdf:about="http://www.theworldavatar.com/ontology/ontopowsys/PowSysFunction.owl">
        <owl:imports rdf:resource="http://www.theworldavatar.com/ontology/ontocape/upper_level/network_system.owl"/>
    </owl:Ontology>
    


    <!-- 
    ///////////////////////////////////////////////////////////////////////////////////////
    //
    // Classes
    //
    ///////////////////////////////////////////////////////////////////////////////////////
     -->

    


    <!-- http://www.theworldavatar.com/ontology/ontopowsys/PowSysFunction.owl#EnergyMetering -->

    <owl:Class rdf:about="http://www.theworldavatar.com/ontology/ontopowsys/PowSysFunction.owl#EnergyMetering">
        <rdfs:subClassOf rdf:resource="http://www.theworldavatar.com/ontology/ontopowsys/PowSysFunction.owl#SystemComponentProcess"/>
        <rdfs:comment>Functionality to observe the energy flowed in a point of an electrical network and visualize it</rdfs:comment>
    </owl:Class>
    


    <!-- http://www.theworldavatar.com/ontology/ontopowsys/PowSysFunction.owl#PowerConsumption -->

    <owl:Class rdf:about="http://www.theworldavatar.com/ontology/ontopowsys/PowSysFunction.owl#PowerConsumption">
        <rdfs:subClassOf rdf:resource="http://www.theworldavatar.com/ontology/ontopowsys/PowSysFunction.owl#SystemComponentProcess"/>
        <rdfs:comment>Functionality to utilize electricity for various purpose</rdfs:comment>
    </owl:Class>
    


    <!-- http://www.theworldavatar.com/ontology/ontopowsys/PowSysFunction.owl#PowerConversion -->

    <owl:Class rdf:about="http://www.theworldavatar.com/ontology/ontopowsys/PowSysFunction.owl#PowerConversion">
        <rdfs:subClassOf rdf:resource="http://www.theworldavatar.com/ontology/ontopowsys/PowSysFunction.owl#PowerFlow"/>
        <rdfs:comment>Functionality to convert electricity from one form to another form</rdfs:comment>
    </owl:Class>
    


    <!-- http://www.theworldavatar.com/ontology/ontopowsys/PowSysFunction.owl#PowerEquipmentConnection -->

    <owl:Class rdf:about="http://www.theworldavatar.com/ontology/ontopowsys/PowSysFunction.owl#PowerEquipmentConnection">
        <rdfs:subClassOf rdf:resource="http://www.theworldavatar.com/ontology/ontopowsys/PowSysFunction.owl#SystemComponentProcess"/>
        <rdfs:comment>Functionality to connect some equipment together in an electrical network system</rdfs:comment>
    </owl:Class>
    


    <!-- http://www.theworldavatar.com/ontology/ontopowsys/PowSysFunction.owl#PowerFlow -->

    <owl:Class rdf:about="http://www.theworldavatar.com/ontology/ontopowsys/PowSysFunction.owl#PowerFlow">
        <rdfs:subClassOf rdf:resource="http://www.theworldavatar.com/ontology/ontopowsys/PowSysFunction.owl#SystemComponentProcess"/>
        <rdfs:comment>Functionality to enable the electrical power to flow from one node to another</rdfs:comment>
    </owl:Class>
    


    <!-- http://www.theworldavatar.com/ontology/ontopowsys/PowSysFunction.owl#PowerGeneration -->

    <owl:Class rdf:about="http://www.theworldavatar.com/ontology/ontopowsys/PowSysFunction.owl#PowerGeneration">
        <rdfs:subClassOf rdf:resource="http://www.theworldavatar.com/ontology/ontopowsys/PowSysFunction.owl#SystemComponentProcess"/>
        <rdfs:comment>Functionality to generate electricity from other type of energy sources</rdfs:comment>
    </owl:Class>
    


    <!-- http://www.theworldavatar.com/ontology/ontopowsys/PowSysFunction.owl#SystemComponentProcess -->

    <owl:Class rdf:about="http://www.theworldavatar.com/ontology/ontopowsys/PowSysFunction.owl#SystemComponentProcess">
        <rdfs:subClassOf rdf:resource="http://www.theworldavatar.com/ontology/ontocape/upper_level/network_system.owl#Device"/>
        <rdfs:comment>A SystemComponent process is a certain network constituent process that operate in the power network</rdfs:comment>
    </owl:Class>
    


    <!-- http://www.theworldavatar.com/ontology/ontopowsys/PowSysFunction.owl#VoltageRegulation -->

    <owl:Class rdf:about="http://www.theworldavatar.com/ontology/ontopowsys/PowSysFunction.owl#VoltageRegulation">
        <rdfs:subClassOf rdf:resource="http://www.theworldavatar.com/ontology/ontopowsys/PowSysFunction.owl#SystemComponentProcess"/>
        <rdfs:comment>Functionality to regulate the voltage level of a system</rdfs:comment>
    </owl:Class>
</rdf:RDF>



<!-- Generated by the OWL API (version 4.2.5.20160517-0735) https://github.com/owlcs/owlapi -->

